pr/347/head/hl/solutions/lean/HL/Equiv.lean
@@ -26,14 +26,13 @@ open scoped HasEval MyGetElem
 --  was very easy to define what it means for a program transformation to
 --  be correct: it should always yield a program that evaluates to the same
 --  number as the original.
-
+--
 --  To talk about the correctness of program transformations for the full
 --  Imp language -- in particular, assignment -- we need to consider the
 --  role of mutable state and develop a more sophisticated notion of
 --  correctness, which we'll call *behavioral equivalence*.
-
+--
 --  For example:
-
 --  - `X + 2` is behaviorally equivalent to `1 + X + 1`
 --  - `X - X` is behaviorally equivalent to `0`
 --  - `(X - 1) + 1` is *not* behaviorally equivalent to `X`
@@ -80,7 +79,7 @@ example : Bexp.Equiv
 --  same ending state whenever they are started in the same initial state,"
 --  because some commands, when run in some starting states, don't
 --  terminate in any final state at all!
-
+--
 --  What we need instead is this: two commands are behaviorally equivalent
 --  if, for any given starting state, they either (1) both diverge or else
 --  (2) both terminate in the same final state. A compact way to express
@@ -130,6 +129,8 @@ theorem skip_right {c : Com} : (imp { ~c; skip }).Equiv c := by
   · intro h
     exact EvalR.seq h EvalR.skip
 
+--  (End of exercise)
+
 --  Similarly, here is a simple equivalence that optimises `if` commands.
 
 theorem if_true_simple {c₁ c₂ : Com} : (imp {if (true) {~c₁} else {~c₂}}).Equiv c₁ := by
@@ -157,42 +158,40 @@ theorem if_true_simple {c₁ c₂ : Com} : (imp {if (true) {~c₁} else {~c₂}}
 --  *Theorem*: If `b` is equivalent to `true`, then
 --  `if (~b) {~c₁}
 --  else {~c₂}` is equivalent to `c₁`. *Proof*:
-
 --  - (`->`) We must show, for all `st` and `st'`, that if
 --    `st =[ imp {if (~b) {~c₁} else {~c₂}} ]=> st'` then
 --    `st =[ c₁ ]=> st'`.
-
+--
 --    Proceed by cases on the rules that could possibly have been used to
 --    show `st =[ imp {if (~b) {~c₁} else {~c₂}} ]=> st'`, namely
 --    `Com.EvalR.ifTrue` and `Com.EvalR.ifFalse`.
-
 --    - Suppose the final rule in the derivation of
 --      `st =[ imp {if (~b) {~c₁} else {~c₂}} ]=> st'` was
 --      `Com.EvalR.ifTrue`. We then have, by the premises of
 --      `Com.EvalR.ifTrue`, that `st =[ c₁ ]=> st'`. This is exactly what
 --      we set out to prove.
-
+--
 --    - On the other hand, suppose the final rule in the derivation of
 --      `st =[ imp {if (~b) {~c₁} else {~c₂}} ]=> st'` was
 --      `Com.EvalR.ifFalse`. We then know that `b.eval st = false` and
 --      `st =[ c₂ ]=> st'`.
-
+--
 --      Recall that `b` is equivalent to `true`, i.e., forall `st`,
 --      `b.eval st = (bexp {true}).eval st`. In particular, this means that
 --      `b.eval st = true`, since `(bexp {true}).eval st = true`. But this
 --      is a contradiction, since `Com.EvalR.ifFalse` requires that
 --      `b.eval st = false`. Thus, the final rule could not have been
 --      `Com.EvalR.ifFalse`.
-
+--
 --  - (`<-`) We must show, for all `st` and `st'`, that if
 --    `st =[ c₁ ]=> st'` then
 --    `st =[ imp {if (~b) {~c₁} else {~c₂}} ]=> st'`.
-
+--
 --    Since `b` is equivalent to `true`, we know that `b.eval st` =
 --    `(bexp {true}).eval st = true` = `true`. Together with the assumption
 --    that `st =[ c₁ ]=> st'`, we can apply `Com.EvalR.ifTrue` to derive
 --    `st =[ imp {if (~b) {~c₁} else {~c₂}} ]=> st'`.
-
+--
 --  Here is the formal version of this proof:
 
 theorem if_true {b : Bexp} {c₁ c₂ : Com} (hb : b.Equiv (bexp {true})) :
@@ -261,11 +260,13 @@ theorem swap_if_branches {b : Bexp} {c₁ c₂ : Com} :
       apply EvalR.ifTrue _ hc
       simp_all
 
+--  (End of exercise)
+
 --  For `while` loops, we can give a similar pair of theorems. A loop whose
 --  guard is equivalent to `false` is equivalent to `skip`, while a loop
 --  whose guard is equivalent to `true` is equivalent to
 --  `while (true) {skip;} end` (or any other non-terminating program).
-
+--
 --  The first of these facts is easy.
 
 theorem while_false_equiv {b : Bexp} {c : Com} (hb : b.Equiv (bexp {false})) :
@@ -285,37 +286,35 @@ theorem while_false_equiv {b : Bexp} {c : Com} (hb : b.Equiv (bexp {false})) :
     apply EvalR.whileFalse
     simp [hb]
 
---  ### Exercise (2 stars): while_false_informal (Advanced, manually graded) ⭐⭐
+--  ### Exercise (2 stars): while_false_informal (Advanced, Manually graded) ⭐⭐
 
 --  Write an informal proof of `while_false_equiv`.
 
+--  (End of exercise)
+
 --  To prove the second fact, we need an auxiliary lemma stating that
 --  `while` loops whose guards are equivalent to `true` never terminate.
-
+--
 --  *Lemma*: If `b` is equivalent to `true`, then it cannot be the case
 --  that `st =[ while (~b) {~c} ]=> st'`.
-
+--
 --  *Proof*: Suppose that `st =[ while (~b) {~c} ]=> st'`. We show, by
 --  induction on a derivation of `st =[ while (~b) {~c} ]=> st'`, that this
 --  assumption leads to a contradiction. The only two cases to consider are
 --  `Com.EvalR.whileFalse` and `Com.EvalR.whileTrue`; the others are
 --  contradictory.
-
 --  - Suppose `st =[ while (~b) {~c} ]=> st'` is proved using rule
 --    `Com.EvalR.whileFalse`. Then by assumption `b.eval st = false`. But
 --    this contradicts the assumption that `b` is equivalent to `true`.
-
+--
 --  - Suppose `st =[ while (~b) {~c} ]=> st'` is proved using rule
 --    `Com.EvalR.whileTrue`. We must have:
-
 --    1. `b.eval st = true`, and
-
 --    2. there is some `st₀` such that `st =[ c ] => st₀` and
 --       `st₀ =[ while (~b) {~c} ]=> st'`.
-
 --    3. Also, we are given an induction hypothesis saying that
 --       `st₀ =[ while (~b) {~c} ]=> st'` leads to a contradiction,
-
+--
 --    We obtain a contradiction by 2 and 3.
 
 theorem while_true_nonterm {b : Bexp} {c : Com} {st st' : State} (hb : b.Equiv (bexp {true})) :
@@ -333,7 +332,7 @@ theorem while_true_nonterm {b : Bexp} {c : Com} {st st' : State} (hb : b.Equiv (
   | skip | asgn | seq | ifTrue | ifFalse =>
     contradiction -- heq says that different commands are equal
 
---  ### Exercise (2 stars): while_true_nonterm_informal (manually graded) ⭐⭐
+--  ### Exercise (2 stars): while_true_nonterm_informal (Manually graded) ⭐⭐
 
 --  Explain what the lemma `while_true_nonterm` means in English.
 
@@ -358,9 +357,11 @@ theorem while_true {b : Bexp} {c : Com} (hb : b.Equiv (bexp {true})) :
     intro
     rfl
 
+--  (End of exercise)
+
 --  A more interesting fact about `while` commands is that any number of
 --  copies of the body can be "unrolled" without changing meaning.
-
+--
 --  Loop unrolling is an important transformation in any real compiler, so
 --  its correctness is of more than just academic interest!
 
@@ -442,6 +443,8 @@ theorem assign_equiv {X : Ident} {a : Aexp} (ha : Aexp.Equiv (aexp {X}) a) :
       simp only [← ha, Aexp.eval_id, TotalMap.update_same]
       exact Com.EvalR.skip
 
+--  (End of exercise)
+
 --  Note to developers (Sati @satiscugcat):
 --      Leaving out optional exercise `equiv_classes` for now.
 
@@ -510,18 +513,18 @@ theorem Com.equiv_trans {c₁ c₂ c₃ : Com} (h₁ : c₁.Equiv c₂) (h₂ : 
 --  Less obviously, behavioral equivalence is also a *congruence*. That is,
 --  the equivalence of two subprograms implies the equivalence of the
 --  larger programs in which they are embedded:
-
+--
 --  aequiv a a' ------------------------- cequiv (x := a) (x := a')
-
+--
 --  cequiv c1 c1' cequiv c2 c2' -------------------------- cequiv (c1;c2)
 --  (c1';c2')
-
+--
 --  ... and so on for the other forms of commands.
-
+--
 --  (Note that we are using the inference rule notation here not as part of
 --  an inductive definition, but simply to write down some valid
 --  implications in a readable format. We prove these implications below.)
-
+--
 --  We will see a concrete example of why these congruence properties are
 --  important in the following section (in the proof of
 --  `fold_constants_com_sound`), but the main idea is that they allow us to
@@ -547,39 +550,37 @@ theorem Com.congruence.asgn {x : Ident} {a a' : Aexp} (ha : a.Equiv a') :
 
 --  The congruence property for loops is a little more interesting, since
 --  it requires induction.
-
+--
 --  *Theorem*: Equivalence is a congruence for `while` -- that is, if `b`
 --  is equivalent to `b'` and `c` is equivalent to `c'`, then
 --  `while (~b) {~c}` is equivalent to `while (~b') {~c'}`.
-
+--
 --  *Proof*: Suppose `b` is equivalent to `b'` and `c` is equivalent to
 --  `c'`. We must show, for every `st` and `st'`, that
 --  `st =[ while (~b) {~c} ]=> st'` iff `st = while (~b') {~c'}
 --  ]=> st'`.
 --  We consider the two directions separately.
-
 --  - (`->`) We show that `st =[ while (~b) {~c} ]=> st'` implies
 --    `st =[ while (~b') {~c'} ]=> st'`, by induction on a derivation of
 --    `st =[ while (~b) {~c} ]=> st'`. The only nontrivial cases are when
 --    the final rule in the derivation is `Com.EvalR.whileFalse` or
 --    `Com.EvalR.whileTrue`.
-
 --    - `Com.EvalR.whileFalse`: In this case, the form of the rule gives us
 --      `beval st b = false` and `st = st'`. But then, since `b` and `b'`
 --      are equivalent, we have `beval st b' =false`, and
 --      `Com.EvalR.whileFalse` applies, giving us
 --      `st =[ while (~b') {~c'} ]=> st'`, as required.
-
+--
 --    - `Com.EvalR.whileTrue`: The form of the rule now gives us
 --      `beval st b = true`, with `st =[ c ]=> st'0` and
 --      `st'0 =[ while {~b} {~c} ]=> st'` for some state `st'0`, with the
 --      induction hypothesis `st'0 =[ while (~b') {~c'} ]=> st'`.
-
+--
 --      Since `c` and `c'` are equivalent, we know that `st =[ c']=> st'0`.
 --      And since `b` and `b'` are equivalent, we have
 --      `beval st b' = true`. Now `Com.EvalR.whileTrue` applies, giving us
 --      `st =[ while (~b') {~c'} ]=> st'`, as required.
-
+--
 --  - (`<-`) Similar.
 
 --  Note to developers (Sati @satiscugcat):
@@ -590,3 +591,4 @@ theorem Com.congruence.asgn {x : Ident} {a a' : Aexp} (ha : a.Equiv a') :
 --        - Extended Exercise: Nondeterministic Imp
 --        - Additional Exercises`
 
+-- Built on 2026-09-10 13:01 UTC
