pr/347/head/ts/solutions/lean/TS.lean
@@ -3,3 +3,8 @@ import TS.Slang
 import TS.Smallstep
 import TS.Types
 import TS.Stlc
+import TS.StlcProp
+import TS.MoreStlc
+import TS.Sub
+
+-- Built on 2026-09-10 13:02 UTC
